\documentclass[aps,onecolumn,pra]{revtex4}
\usepackage{amsmath}
\usepackage{amsfonts}
\usepackage{bm}
\begin{document}
    \begin{eqnarray}
		B_1 (\bm{\Delta}) & = & \overline{u(\bm{r}+\bm{\Delta})^2 - u(\bm{r})^2}, \\
		B_2 (\bm{\Delta}) & = & \overline{\left[
				u(\bm{r}+\bm{\Delta})-u(\bm{r})
			\right]^2}
    \end{eqnarray}
    \begin{eqnarray}
		\left[B_i\right] & = & \left( L T^{-1} \right)^2 = L^2 T^{-2}, \\
		\left[\epsilon\right] & = & \left( L^2 T^{-2} \right)T^{-1} = L^2 T^{-3}, \\
		\left[\bm{\Delta}\right] & = & L
    \end{eqnarray}
    \begin{eqnarray}
		\left\{
			\begin{array}{l}
				\epsilon = \frac{E(\bm{r})}{m}/t = L^2 T^{-2} / T = L^2 T^{-3}, \ {\rm unit \ of \ power}
				\\
				\bm{\Delta} = L
			\end{array}
		\right.
    \end{eqnarray}
    \begin{eqnarray}
		\epsilon \bm{\Delta} & = & (L^2 T^{-3})L = L^3 T^{-3} \\
		\frac{E(\bm{r})}{m} & = & L^2 T^{-2} \\
		B_i(\bm{r}) & = & \epsilon^{\frac{2}{3}} \bm{\Delta}^{\frac{2}{3}} = L^{3 \frac{2}{3}} T^{-3 \frac{2}{3}} = L^2 T^{-2} = \frac{E(\bm{r})}{m}
    \end{eqnarray}
    \begin{eqnarray}
		B_i(\bm{k}) & = & \frac{1}{2 \pi} \int B_i(\bm{r}) e^{i \bm{k} \bm{r}} d\bm{r}
		\\
		& \propto & C \epsilon^{\frac{2}{3}} \bm{\Delta}^{1 + \frac{2}{3}} = \epsilon^{\frac{2}{3}} \bm{\Delta}^{\frac{5}{3}}
		\\
		& \propto & C \epsilon^{\frac{2}{3}} \bm{k}^{-\frac{5}{3}}
    \end{eqnarray}
\end{document}
